NumLean/Data/KernelExpr/Basic.lean
@@ -1,0 +1,228 @@
+import NumLean.Algebra.Float
+
+namespace NumLean
+
+inductive KernelTypeTag where
+  | real
+  | nat
+  | int
+deriving Repr, BEq
+
+abbrev KernelType (R : Type) : KernelTypeTag -> Type
+  | .real => R
+  | .nat => Nat
+  | .int => Int
+
+/-- Well-typed scalar/index expression syntax for kernels. -/
+inductive KernelExpr (R : Type) : KernelTypeTag -> Type where
+  | bvar (t : KernelTypeTag) (idx : Nat) : KernelExpr R t
+  | ctx (arrayIndex : Nat) (elemIndex : KernelExpr R .nat) : KernelExpr R .real
+  | ctxSize (arrayIndex : Nat) : KernelExpr R .nat
+  | lit (v : R) : KernelExpr R .real
+  | natLit (v : Nat) : KernelExpr R .nat
+  | intLit (v : Int) : KernelExpr R .int
+  | cast (t : KernelTypeTag) {s : KernelTypeTag} (a : KernelExpr R s) : KernelExpr R t
+  | add {t} (a b : KernelExpr R t) : KernelExpr R t
+  | sub {t} (a b : KernelExpr R t) : KernelExpr R t
+  | mul {t} (a b : KernelExpr R t) : KernelExpr R t
+  | div {t} (a b : KernelExpr R t) : KernelExpr R t
+  | neg {t} (a : KernelExpr R t) : KernelExpr R t
+  | abs {t} (a : KernelExpr R t) : KernelExpr R t
+  | sqrt (a : KernelExpr R .real) : KernelExpr R .real
+  | sin (a : KernelExpr R .real) : KernelExpr R .real
+  | cos (a : KernelExpr R .real) : KernelExpr R .real
+  | exp (a : KernelExpr R .real) : KernelExpr R .real
+  | log (a : KernelExpr R .real) : KernelExpr R .real
+  | fma (a b c : KernelExpr R .real) : KernelExpr R .real
+  | min {t} (a b : KernelExpr R t) : KernelExpr R t
+  | max {t} (a b : KernelExpr R t) : KernelExpr R t
+  | ifLt {c t} (a b : KernelExpr R c) (thenExpr elseExpr : KernelExpr R t) : KernelExpr R t
+deriving Repr
+
+namespace KernelExpr
+
+instance : Add (KernelExpr R t) where add := .add
+instance : Sub (KernelExpr R t) where sub := .sub
+instance : Mul (KernelExpr R t) where mul := .mul
+instance : Div (KernelExpr R t) where div := .div
+instance : Neg (KernelExpr R t) where neg := .neg
+
+def WellFormed (boundVars : Array ((t : KernelTypeTag) × KernelType R t)) (ctx : Array (Array R)) :
+    KernelExpr R t -> Prop
+  | .bvar t i => ∃ h : i < boundVars.size, (boundVars[i]'h).1 = t
+  | .ctx arrayIndex elemIndex => arrayIndex < ctx.size ∧ WellFormed boundVars ctx elemIndex
+  | .ctxSize arrayIndex => arrayIndex < ctx.size
+  | .lit _ | .natLit _ | .intLit _ => True
+  | .cast _ a | .neg a | .abs a |
+      .sqrt a | .sin a | .cos a | .exp a | .log a => WellFormed boundVars ctx a
+  | .add a b | .sub a b | .mul a b | .div a b | .min a b | .max a b =>
+      WellFormed boundVars ctx a ∧ WellFormed boundVars ctx b
+  | .fma a b c => WellFormed boundVars ctx a ∧ WellFormed boundVars ctx b ∧ WellFormed boundVars ctx c
+  | .ifLt a b thenExpr elseExpr =>
+      WellFormed boundVars ctx a ∧
+      WellFormed boundVars ctx b ∧
+      WellFormed boundVars ctx thenExpr ∧
+      WellFormed boundVars ctx elseExpr
+
+instance [Add R] : Add (KernelType R t) := match t with
+  | .real => inferInstanceAs (Add R)
+  | .int => inferInstanceAs (Add Int)
+  | .nat => inferInstanceAs (Add Nat)
+
+def eval {R : Type} [ROps R] [DecidableRel (· < · : R -> R -> Prop)]
+    (boundVars : Array ((t : KernelTypeTag) × KernelType R t))
+    (ctx : Array (Array R)) {t} (k : KernelExpr R t)
+    (hk : WellFormed boundVars ctx k) :
+    KernelType R t :=
+  match t, k with
+  | _, .bvar _ i =>
+    let val := boundVars[i]'(by simp [WellFormed] at hk; grind)
+    _root_.cast (by simp [WellFormed] at hk; obtain ⟨_,hk⟩ := hk; rw[hk]) val.2
+  | _, .ctx arrayIndex elemIndex =>
+    have idx := elemIndex.eval boundVars ctx hk.2
+    (ctx[arrayIndex]'hk.1).getD idx 0
+  | _, .ctxSize arrayIndex =>
+    (ctx[arrayIndex]'hk).size
+  | _, .lit v => v
+  | _, .natLit v => v
+  | _, .intLit v => v
+  | .real, .cast _ (s := .real) a =>
+    a.eval boundVars ctx (by simpa [WellFormed] using hk)
+  | .real, .cast _ (s := .nat) a =>
+    a.eval boundVars ctx (by simpa [WellFormed] using hk) • (1 : R)
+  | .real, .cast _ (s := .int) a =>
+    a.eval boundVars ctx (by simpa [WellFormed] using hk) • (1 : R)
+  | .nat, .cast _ (s := .real) _ =>
+    0
+  | .nat, .cast _ (s := .nat) a =>
+    a.eval boundVars ctx (by simpa [WellFormed] using hk)
+  | .nat, .cast _ (s := .int) a =>
+    (a.eval boundVars ctx (by simpa [WellFormed] using hk)).toNat
+  | .int, .cast _ (s := .real) _ =>
+    0
+  | .int, .cast _ (s := .nat) a =>
+    Int.ofNat (a.eval boundVars ctx (by simpa [WellFormed] using hk))
+  | .int, .cast _ (s := .int) a =>
+    a.eval boundVars ctx (by simpa [WellFormed] using hk)
+  | _, add x y =>
+    x.eval boundVars ctx hk.1 + y.eval boundVars ctx hk.2
+  | .real, sub x y =>
+    x.eval boundVars ctx hk.1 - y.eval boundVars ctx hk.2
+  | .nat, sub x y =>
+    x.eval boundVars ctx hk.1 - y.eval boundVars ctx hk.2
+  | .int, sub x y =>
+    x.eval boundVars ctx hk.1 - y.eval boundVars ctx hk.2
+  | .real, mul x y =>
+    x.eval boundVars ctx hk.1 * y.eval boundVars ctx hk.2
+  | .nat, mul x y =>
+    x.eval boundVars ctx hk.1 * y.eval boundVars ctx hk.2
+  | .int, mul x y =>
+    x.eval boundVars ctx hk.1 * y.eval boundVars ctx hk.2
+  | .real, div x y =>
+    x.eval boundVars ctx hk.1 / y.eval boundVars ctx hk.2
+  | .nat, div x y =>
+    x.eval boundVars ctx hk.1 / y.eval boundVars ctx hk.2
+  | .int, div x y =>
+    x.eval boundVars ctx hk.1 / y.eval boundVars ctx hk.2
+  | .real, neg x =>
+    -x.eval boundVars ctx (by simpa [WellFormed] using hk)
+  | .nat, neg x =>
+    x.eval boundVars ctx (by simpa [WellFormed] using hk)
+  | .int, neg x =>
+    -x.eval boundVars ctx (by simpa [WellFormed] using hk)
+  | .real, abs x =>
+    let v := x.eval boundVars ctx (by simpa [WellFormed] using hk)
+    if v < 0 then -v else v
+  | .nat, abs x =>
+    x.eval boundVars ctx (by simpa [WellFormed] using hk)
+  | .int, abs x =>
+    let v := x.eval boundVars ctx (by simpa [WellFormed] using hk)
+    if v < 0 then -v else v
+  | _, sqrt x =>
+    ROps.sqrt (x.eval boundVars ctx (by simpa [WellFormed] using hk))
+  | _, sin x =>
+    RCOps.sin (x.eval boundVars ctx (by simpa [WellFormed] using hk))
+  | _, cos x =>
+    RCOps.cos (x.eval boundVars ctx (by simpa [WellFormed] using hk))
+  | _, exp x =>
+    RCOps.exp (x.eval boundVars ctx (by simpa [WellFormed] using hk))
+  | _, log x =>
+    ROps.log (x.eval boundVars ctx (by simpa [WellFormed] using hk))
+  | _, fma x y z =>
+    x.eval boundVars ctx hk.1 * y.eval boundVars ctx hk.2.1 + z.eval boundVars ctx hk.2.2
+  | .real, min x y =>
+    let xv := x.eval boundVars ctx hk.1
+    let yv := y.eval boundVars ctx hk.2
+    if xv < yv then xv else yv
+  | .nat, min x y =>
+    Nat.min (x.eval boundVars ctx hk.1) (y.eval boundVars ctx hk.2)
+  | .int, min x y =>
+    let xv := x.eval boundVars ctx hk.1
+    let yv := y.eval boundVars ctx hk.2
+    if xv < yv then xv else yv
+  | .real, max x y =>
+    let xv := x.eval boundVars ctx hk.1
+    let yv := y.eval boundVars ctx hk.2
+    if xv < yv then yv else xv
+  | .nat, max x y =>
+    Nat.max (x.eval boundVars ctx hk.1) (y.eval boundVars ctx hk.2)
+  | .int, max x y =>
+    let xv := x.eval boundVars ctx hk.1
+    let yv := y.eval boundVars ctx hk.2
+    if xv < yv then yv else xv
+  | _, ifLt (c := .real) a b x y =>
+    if a.eval boundVars ctx hk.1 < b.eval boundVars ctx hk.2.1 then
+      x.eval boundVars ctx hk.2.2.1
+    else
+      y.eval boundVars ctx hk.2.2.2
+  | _, ifLt (c := .nat) a b x y =>
+    if a.eval boundVars ctx hk.1 < b.eval boundVars ctx hk.2.1 then
+      x.eval boundVars ctx hk.2.2.1
+    else
+      y.eval boundVars ctx hk.2.2.2
+  | _, ifLt (c := .int) a b x y =>
+    if a.eval boundVars ctx hk.1 < b.eval boundVars ctx hk.2.1 then
+      x.eval boundVars ctx hk.2.2.1
+    else
+      y.eval boundVars ctx hk.2.2.2
+termination_by sizeOf k
+
+
+def toCCodeBody {R} [ToString R] {t} (k : KernelExpr R t) : String :=
+  match k with
+  | .bvar _ idx => s!"x{idx}"
+  | .ctx arrayIndex elemIndex => s!"hy{arrayIndex}[{toCCodeBody elemIndex}]"
+  | .ctxSize arrayIndex => s!"hy{arrayIndex}_size"
+  | .lit v => s!"{v}"
+  | .natLit v => s!"{v}"
+  | .intLit v => s!"{v}"
+  | .cast .real a => s!"((float)({toCCodeBody a}))"
+  | .cast .nat a => s!"((size_t)({toCCodeBody a}))"
+  | .cast .int a => s!"((long)({toCCodeBody a}))"
+  | .add a b => s!"({toCCodeBody a} + {toCCodeBody b})"
+  | .sub a b => s!"({toCCodeBody a} - {toCCodeBody b})"
+  | .mul a b => s!"({toCCodeBody a} * {toCCodeBody b})"
+  | .div a b => s!"({toCCodeBody a} / {toCCodeBody b})"
+  | .neg a => s!"(-{toCCodeBody a})"
+  | .abs a => s!"abs({toCCodeBody a})"
+  | .sqrt a => s!"sqrt({toCCodeBody a})"
+  | .sin a => s!"sin({toCCodeBody a})"
+  | .cos a => s!"cos({toCCodeBody a})"
+  | .exp a => s!"exp({toCCodeBody a})"
+  | .log a => s!"log({toCCodeBody a})"
+  | .fma a b c => s!"fma({toCCodeBody a}, {toCCodeBody b}, {toCCodeBody c})"
+  | .min a b => s!"min({toCCodeBody a}, {toCCodeBody b})"
+  | .max a b => s!"max({toCCodeBody a}, {toCCodeBody b})"
+  | .ifLt a b thenExpr elseExpr =>
+    s!"(({toCCodeBody a} < {toCCodeBody b}) ? {toCCodeBody thenExpr} : {toCCodeBody elseExpr})"
+
+
+
+-- def eval (ctx : Array (Array Float32)) (x : Float32) (gid : Nat) (expr : Float32KernelExpr) : Float32 :=
+--   KernelExpr.eval ctx x gid expr
+
+-- def mapArraySpec (expr : Float32KernelExpr) (ctx : Array (Array Float32)) (xs : Array Float32) : Array Float32 :=
+--   KernelExpr.mapArraySpec expr ctx xs
+
+end KernelExpr
+end NumLean
