NumLean/Data/KernelExpr/Register.lean
@@ -1,0 +1,9 @@
+import NumLean.Tactic.ApplyRuleSets
+
+open NumLean.Tactic.ApplyRuleSets
+
+namespace NumLean
+
+register_ruleset compile_kernel_expr
+
+end NumLean
