NumLean/Data/TensorIndex.lean
@@ -1,4 +1,6 @@
 import NumLean.Data.TensorIndex.Basic
 import NumLean.Data.TensorIndex.Dense
+import NumLean.Data.TensorIndex.Hierarchical
+import NumLean.Data.TensorIndex.Linear
 import NumLean.Data.TensorIndex.TensorIndexType
 import NumLean.Data.TensorIndex.TensorSliceMap
